#+TITLE: Weeek4
#+AUTHOR: 陈淇奥@@latex:\\@@21210160025
#+OPTIONS: toc:nil
#+LATEX_HEADER: \input{../../../preamble-lite.tex}
#+LATEX_HEADER: \usepackage[UTF8]{ctex}

#+ATTR_LATEX: :options [1.2.10]
#+BEGIN_exercise
假设\(G=\{g\}\subseteq B\),\(F\)是由\(G\)生成的滤，则以下命题等价
1. \(g\)是原子
2. \(F\)是超滤
3. \(F\)是主超滤
#+END_exercise

#+BEGIN_proof
\(1\to 2\): 因为\(g\)是原子，对任意\(b\in B\),\(b\neq 0\)，\(a\le b\)或者\(a\le -b\)且不同时成立，于是\(b\in F\)
或者\(-b\in F\)，因此\(F\)是超滤

\(2\to 3\): 因为\(F\)由单点集生成

\(3\to 1\): 对于任意\(b\in B\),\(b\neq 0\)，有\(b\in F\)或\(-b\in F\)，于是\(g\le b\)或\(g\le -b\)，且\(b,-b\)不会
同时属于超滤，因此\(g\)是原子
#+END_proof

#+ATTR_LATEX: :options [1.2.13]
#+BEGIN_exercise
\(F\)是\(\calb\)上的滤当且仅当\(I=\{-a\mid a\in F\}\)是\(\calb\)上的理想
#+END_exercise

#+BEGIN_proof
\(\Rightarrow\): 因为\(F\)是\(B\)上的滤，因此\(1\in F\),\(0\notin F\)，于是\(0\in I\), \(1\notin F\)。如果\(a,b\in I\),于
是\(-a,-b\in F\)，因此\((-a)\cdot(-b)\in F\)，因此\(a+b\in I\)。如果\(a\in I\)且\(b\le a\)，则\(-a\in F\)，
\(-a\le -b\)，于是\(-b\in F\)，因此\(b\in I\)。因此\(I\)是理想

\(\Leftarrow\): 因为\(I\)是理想，\(1\notin I\),\(0\in I\)，于是\(1\in F\), \(0\notin F\)。若\(a,b\in F\)，则\(-a,-b\in I\),于
是\(-a+-b\in I\)，因此\(a\cdot b\in F\)。若\(a\in F\)且\(a\le b\)，则\(-a\in I\)且\(-b\le -a\)，于是\(-b\in I\)，因
而\(b\in F\)。因此\(F\)是\(\calb\)上的滤
#+END_proof

#+ATTR_LATEX: :options [1.2.17]
#+BEGIN_exercise
令\(\calb\)是布尔代数，\(a,b\in B\)
1. \(a\triangle a=0\)
2. \(a\triangle b=b\triangle a\)
3. \(a\triangledown b=-(-a\triangle-b)\)
#+END_exercise

#+BEGIN_proof
1. \(a\triangle a=(a\cdot(-a))+(a\cdot(-a))=0+0=0\)
2. \(a\triangle b=(a\cdot(-b))+(b\cdot(-a))=(b\cdot(-a))+(a\cdot(-b))=b\triangle a\)
3. \(-(-a\triangle-b)=-(a\cdot(-b))+(b\cdot(-a))=(-a+b)\cdot(-b+a)=a\triangledown b\)
#+END_proof

#+ATTR_LATEX: :options [1.2.20]
#+BEGIN_exercise
\(a\sim_Fb\)当且仅当\(c\in F\), \(c\cdot a=c\cdot b\)
#+END_exercise

#+BEGIN_proof
\(a\sim_Fb\)当且仅当\((a+(-b))\cdot(b+(-a))\in F\)当且仅当\(a+(-b),b+(-a)\in F\)

\(\Rightarrow\): 因为\(a\sim_Fb\)，因此\(ab+(-a)(-b)\in F\)，令\(c=ab+(-a)(-b)\)，则\(ca=ab=cb\)

\(\Leftarrow\): 因为\(c(a+(-b))=ca+c(-b)=cb+c(-b)=c\in F\)，因此\((a+(-b))\in F\)，同理\(b+(-a)\in F\)，因此\(a\sim_Fb\)
#+END_proof

#+ATTR_LATEX: :options [1.2.26]
#+BEGIN_exercise
如果\(a\neq b\)，则存在超滤\(U\),\(a\in U\)但\(b\notin U\)，或者\(b\in U\)但是\(a\notin U\)
#+END_exercise

#+BEGIN_proof
若\(a(-b)\neq 0\)，则存在超滤\(U\supseteq\{a(-b)\}\)，于是\(a\in U\),\(-b\in U\)

若\(a(-b)=0=(-a)b\)，则\(a+(-b)=1\)，于是\(-b=-a\)，因此\(a=b\)矛盾。于是若\(a(-b)=0\)，则\((-a)b\neq 0\)，则存在超
滤\(U'\supseteq\{(-a)b\}\)，于是\(a\notin U'\),\(b\in U\)
#+END_proof
